coq-menhirlib/src/Validator_safe.v
@@ -11,9 +11,10 @@
 (*                                                                          *)
 (****************************************************************************)
 
-From Coq Require Import List Syntax.
+From Coq Require Import List Syntax Derive.
+From Coq.ssr Require Import ssreflect.
 Require Automaton.
-Require Import Alphabet.
+Require Import Alphabet Validator_classes.
 
 Module Make(Import A:Automaton.T).
 
@@ -24,16 +25,16 @@ Definition singleton_state_pred (state:state) :=
 (** [past_state_of_non_init_state], extended for all states. **)
 Definition past_state_of_state (state:state) :=
   match state with
-    | Init _ => []
-    | Ninit nis => past_state_of_non_init_state nis
+  | Init _ => []
+  | Ninit nis => past_state_of_non_init_state nis
   end.
 
 (** Concatenations of last and past **)
 Definition head_symbs_of_state (state:state) :=
   match state with
-    | Init _ => []
-    | Ninit s =>
-      last_symb_of_non_init_state s::past_symb_of_non_init_state s
+  | Init _ => []
+  | Ninit s =>
+    last_symb_of_non_init_state s::past_symb_of_non_init_state s
   end.
 Definition head_states_of_state (state:state) :=
   singleton_state_pred state::past_state_of_state state.
@@ -42,38 +43,30 @@ Definition head_states_of_state (state:state) :=
 
 (** Prefix predicate between two lists of symbols. **)
 Inductive prefix: list symbol -> list symbol -> Prop :=
-  | prefix_nil: forall l, prefix [] l
-  | prefix_cons: forall l1 l2 x, prefix l1 l2 -> prefix (x::l1) (x::l2).
+| prefix_nil: forall l, prefix [] l
+| prefix_cons: forall l1 l2 x, prefix l1 l2 -> prefix (x::l1) (x::l2).
 
-(** [prefix] is associative **)
-Lemma prefix_ass:
+(** [prefix] is transitive **)
+Lemma prefix_trans:
   forall (l1 l2 l3:list symbol), prefix l1 l2 -> prefix l2 l3 -> prefix l1 l3.
 Proof.
   intros l1 l2 l3 H1 H2. revert l3 H2.
   induction H1; [now constructor|]. inversion 1. subst. constructor. eauto.
 Qed.
 
-Fixpoint is_prefix (l1 l2:list symbol):=
+Fixpoint is_prefix (l1 l2:list symbol) :=
   match l1, l2 with
-    | [], _ => true
-    | t1::q1, t2::q2 => (compare_eqb t1 t2 && is_prefix q1 q2)%bool
-    | _::_, [] => false
+  | [], _ => true
+  | t1::q1, t2::q2 => (compare_eqb t1 t2 && is_prefix q1 q2)%bool
+  | _::_, [] => false
   end.
 
-Property is_prefix_correct (l1 l2:list symbol):
-  is_prefix l1 l2 = true -> prefix l1 l2.
+Instance prefix_is_validator l1 l2 : IsValidator (prefix l1 l2) (is_prefix l1 l2).
 Proof.
-revert l2.
-induction l1; intros.
-apply prefix_nil.
-unfold is_prefix in H.
-destruct l2; intuition; try discriminate.
-rewrite Bool.andb_true_iff in H.
-destruct H.
-rewrite compare_eqb_iff in H.
-destruct H.
-apply prefix_cons.
-apply IHl1; intuition.
+  revert l2. induction l1 as [|x1 l1 IH]=>l2 Hpref.
+  - constructor.
+  - destruct l2 as [|x2 l2]=>//.
+    move: Hpref=> /andb_prop [/compare_eqb_iff -> /IH ?]. by constructor.
 Qed.
 
 (** If we shift, then the known top symbols of the destination state is
@@ -82,43 +75,14 @@ Qed.
 Definition shift_head_symbs :=
   forall s,
     match action_table s with
-      | Lookahead_act awp =>
-        forall t, match awp t with
-          | Shift_act s2 _ =>
-            prefix (past_symb_of_non_init_state s2) (head_symbs_of_state s)
-          | _ => True
+    | Lookahead_act awp => forall t,
+        match awp t with
+        | Shift_act s2 _ =>
+          prefix (past_symb_of_non_init_state s2) (head_symbs_of_state s)
+        | _ => True
         end
-      | _ => True
+    | _ => True
     end.
-
-Definition is_shift_head_symbs (_:unit) :=
-  forallb (fun s:state =>
-    match action_table s with
-      | Lookahead_act awp =>
-        forallb (fun t =>
-          match awp t with
-            | Shift_act s2 _ =>
-              is_prefix (past_symb_of_non_init_state s2) (head_symbs_of_state s)
-            | _ => true
-          end)
-          all_list
-      | _ => true
-    end)
-    all_list.
-
-Property is_shift_head_symbs_correct:
-  is_shift_head_symbs () = true -> shift_head_symbs.
-Proof.
-unfold is_shift_head_symbs, shift_head_symbs.
-intros.
-rewrite forallb_forall in H.
-specialize (H s (all_list_forall s)).
-destruct (action_table s); intuition.
-rewrite forallb_forall in H.
-specialize (H t (all_list_forall t)).
-destruct (l t); intuition.
-apply is_prefix_correct; intuition.
-Qed.
 
 (** When a goto happens, then the known top symbols of the destination state
     is a prefix of the known top symbols of the source state, with the new
@@ -126,35 +90,10 @@ Qed.
 Definition goto_head_symbs :=
   forall s nt,
     match goto_table s nt with
-      | Some (exist _ s2 _) =>
-        prefix (past_symb_of_non_init_state s2) (head_symbs_of_state s)
-      | None => True
+    | Some (exist _ s2 _) =>
+      prefix (past_symb_of_non_init_state s2) (head_symbs_of_state s)
+    | None => True
     end.
-
-Definition is_goto_head_symbs (_:unit) :=
-  forallb (fun s:state =>
-    forallb (fun nt =>
-      match goto_table s nt with
-        | Some (exist _ s2 _) =>
-          is_prefix (past_symb_of_non_init_state s2) (head_symbs_of_state s)
-        | None => true
-      end)
-      all_list)
-    all_list.
-
-Property is_goto_head_symbs_correct:
-  is_goto_head_symbs () = true -> goto_head_symbs.
-Proof.
-unfold is_goto_head_symbs, goto_head_symbs.
-intros.
-rewrite forallb_forall in H.
-specialize (H s (all_list_forall s)).
-rewrite forallb_forall in H.
-specialize (H nt (all_list_forall nt)).
-destruct (goto_table s nt); intuition.
-destruct s0.
-apply is_prefix_correct; intuition.
-Qed.
 
 (** We have to say the same kind of checks for the assumptions about the
     states stack. However, theses assumptions are predicates. So we define
@@ -166,8 +105,8 @@ Inductive prefix_pred: list (state->bool) -> list (state->bool) -> Prop :=
      (forall x, implb (f2 x) (f1 x) = true) ->
      prefix_pred l1 l2 -> prefix_pred (f1::l1) (f2::l2).
 
-(** [prefix_pred] is associative **)
-Lemma prefix_pred_ass:
+(** [prefix_pred] is transitive **)
+Lemma prefix_pred_trans:
   forall (l1 l2 l3:list (state->bool)),
   prefix_pred l1 l2 -> prefix_pred l2 l3 -> prefix_pred l1 l3.
 Proof.
@@ -180,109 +119,46 @@ Qed.
 
 Fixpoint is_prefix_pred (l1 l2:list (state->bool)) :=
   match l1, l2 with
-    | [], _ => true
-    | f1::q1, f2::q2 =>
-      (forallb (fun x => implb (f2 x) (f1 x)) all_list
-        && is_prefix_pred q1 q2)%bool
-    | _::_, [] => false
+  | [], _ => true
+  | f1::q1, f2::q2 =>
+    (forallb (fun x => implb (f2 x) (f1 x)) all_list
+      && is_prefix_pred q1 q2)%bool
+  | _::_, [] => false
   end.
 
-Property is_prefix_pred_correct (l1 l2:list (state->bool)) :
-  is_prefix_pred l1 l2 = true -> prefix_pred l1 l2.
+Instance prefix_pred_is_validator l1 l2 :
+  IsValidator (prefix_pred l1 l2) (is_prefix_pred l1 l2).
 Proof.
-revert l2.
-induction l1.
-intros.
-apply prefix_pred_nil.
-intros.
-destruct l2; intuition; try discriminate.
-unfold is_prefix_pred in H.
-rewrite Bool.andb_true_iff in H.
-rewrite forallb_forall in H.
-apply prefix_pred_cons; intuition.
-apply H0.
-apply all_list_forall.
+  revert l2. induction l1 as [|x1 l1 IH]=>l2 Hpref.
+  - constructor.
+  - destruct l2 as [|x2 l2]=>//.
+    move: Hpref=> /andb_prop [/forallb_forall ? /IH ?].
+    constructor; auto using all_list_forall.
 Qed.
 
 (** The assumptions about state stack is conserved when we shift **)
 Definition shift_past_state :=
   forall s,
     match action_table s with
-      | Lookahead_act awp =>
-        forall t, match awp t with
-          | Shift_act s2 _ =>
-            prefix_pred (past_state_of_non_init_state s2)
-                        (head_states_of_state s)
-          | _ => True
+    | Lookahead_act awp => forall t,
+        match awp t with
+        | Shift_act s2 _ =>
+          prefix_pred (past_state_of_non_init_state s2)
+                      (head_states_of_state s)
+        | _ => True
         end
-      | _ => True
+    | _ => True
     end.
-
-Definition is_shift_past_state (_:unit) :=
-  forallb (fun s:state =>
-    match action_table s with
-      | Lookahead_act awp =>
-        forallb (fun t =>
-          match awp t with
-            | Shift_act s2 _ =>
-              is_prefix_pred
-                (past_state_of_non_init_state s2) (head_states_of_state s)
-            | _ => true
-          end)
-          all_list
-      | _ => true
-    end)
-    all_list.
-
-Property is_shift_past_state_correct:
- is_shift_past_state () = true -> shift_past_state.
-Proof.
-unfold is_shift_past_state, shift_past_state.
-intros.
-rewrite forallb_forall in H.
-specialize (H s (all_list_forall s)).
-destruct (action_table s); intuition.
-rewrite forallb_forall in H.
-specialize (H t (all_list_forall t)).
-destruct (l t); intuition.
-apply is_prefix_pred_correct; intuition.
-Qed.
 
 (** The assumptions about state stack is conserved when we do a goto **)
 Definition goto_past_state :=
   forall s nt,
     match goto_table s nt with
-      | Some (exist _ s2 _) =>
-        prefix_pred (past_state_of_non_init_state s2)
-                    (head_states_of_state s)
-      | None => True
+    | Some (exist _ s2 _) =>
+      prefix_pred (past_state_of_non_init_state s2)
+                  (head_states_of_state s)
+    | None => True
     end.
-
-Definition is_goto_past_state (_:unit) :=
-  forallb (fun s:state =>
-    forallb (fun nt =>
-      match goto_table s nt with
-        | Some (exist _ s2 _) =>
-          is_prefix_pred
-            (past_state_of_non_init_state s2) (head_states_of_state s)
-        | None => true
-      end)
-      all_list)
-    all_list.
-
-Property is_goto_past_state_correct :
-  is_goto_past_state () = true -> goto_past_state.
-Proof.
-unfold is_goto_past_state, goto_past_state.
-intros.
-rewrite forallb_forall in H.
-specialize (H s (all_list_forall s)).
-rewrite forallb_forall in H.
-specialize (H nt (all_list_forall nt)).
-destruct (goto_table s nt); intuition.
-destruct s0.
-apply is_prefix_pred_correct; intuition.
-Qed.
 
 (** What states are possible after having popped these symbols from the
     stack, given the annotation of the current state ? **)
@@ -296,20 +172,22 @@ Inductive state_valid_after_pop (s:state):
     forall st sq p pl, state_valid_after_pop s sq pl ->
       state_valid_after_pop s (st::sq) (p::pl).
 
-Fixpoint is_state_valid_after_pop
-  (state:state) (to_pop:list symbol) annot :=
+Fixpoint is_state_valid_after_pop (state:state) (to_pop:list symbol) annot :=
   match annot, to_pop with
-    | [], _ => true
-    | p::_, [] => p state
-    | p::pl, s::sl => is_state_valid_after_pop state sl pl
+  | [], _ => true
+  | p::_, [] => p state
+  | p::pl, s::sl => is_state_valid_after_pop state sl pl
   end.
 
-Property is_state_valid_after_pop_complete state sl pl :
-  state_valid_after_pop state sl pl -> is_state_valid_after_pop state sl pl = true.
+Instance impl_is_state_valid_after_pop_is_validator state sl pl P b :
+  IsValidator P b ->
+  IsValidator (state_valid_after_pop state sl pl -> P)
+              (if is_state_valid_after_pop state sl pl then b else true).
 Proof.
-intro.
-induction H; intuition.
-destruct sl; intuition.
+  destruct (is_state_valid_after_pop state0 sl pl) eqn:EQ.
+  - intros ??. auto using is_validator.
+  - intros _ _ Hsvap. exfalso. induction Hsvap=>//; [simpl in EQ; congruence|].
+    by destruct sl.
 Qed.
 
 (** A state is valid for reducing a production when :
@@ -322,110 +200,35 @@ Definition valid_for_reduce (state:state) prod :=
     forall state_new,
     state_valid_after_pop state_new
       (prod_rhs_rev prod) (head_states_of_state state) ->
-    goto_table state_new (prod_lhs prod) = None ->
-    match state_new with
+    match goto_table state_new (prod_lhs prod) with
+    | None =>
+      match state_new with
       | Init i => prod_lhs prod = start_nt i
       | Ninit _ => False
+      end
+    | _ => True
     end.
-
-Definition is_valid_for_reduce (state:state) prod:=
-  (is_prefix (prod_rhs_rev prod) (head_symbs_of_state state) &&
-   forallb (fun state_new =>
-     if is_state_valid_after_pop state_new (prod_rhs_rev prod)
-                                           (head_states_of_state state) then
-       match goto_table state_new (prod_lhs prod) with
-         | Some _ => true
-         | None =>
-           match state_new with
-             | Init i => compare_eqb (prod_lhs prod) (start_nt i)
-             | Ninit _ => false
-           end
-       end
-     else
-       true)
-     all_list)%bool.
-
-Property is_valid_for_reduce_correct (state:state) prod:
-  is_valid_for_reduce state prod = true -> valid_for_reduce state prod.
-Proof.
-unfold is_valid_for_reduce, valid_for_reduce.
-intros.
-rewrite Bool.andb_true_iff in H.
-split.
-apply is_prefix_correct.
-intuition.
-intros.
-rewrite forallb_forall in H.
-destruct H.
-specialize (H2 state_new (all_list_forall state_new)).
-rewrite is_state_valid_after_pop_complete, H1 in H2.
-destruct state_new; intuition.
-rewrite compare_eqb_iff in H2; intuition.
-intuition.
-Qed.
 
 (** All the states that does a reduce are valid for reduction **)
 Definition reduce_ok :=
   forall s,
     match action_table s with
-      | Lookahead_act awp =>
-        forall t, match awp t with
-          | Reduce_act p => valid_for_reduce s p
-          | _ => True
-        end
-      | Default_reduce_act p => valid_for_reduce s p
+    | Lookahead_act awp =>
+      forall t, match awp t with
+                | Reduce_act p => valid_for_reduce s p
+                | _ => True
+                end
+    | Default_reduce_act p => valid_for_reduce s p
     end.
-
-Definition is_reduce_ok (_:unit) :=
-  forallb (fun s =>
-    match action_table s with
-      | Lookahead_act awp =>
-        forallb (fun t =>
-          match awp t with
-            | Reduce_act p => is_valid_for_reduce s p
-            | _ => true
-          end)
-          all_list
-      | Default_reduce_act p => is_valid_for_reduce s p
-    end)
-    all_list.
-
-Property is_reduce_ok_correct :
-  is_reduce_ok () = true -> reduce_ok.
-Proof.
-unfold is_reduce_ok, reduce_ok.
-intros.
-rewrite forallb_forall in H.
-specialize (H s (all_list_forall s)).
-destruct (action_table s).
-apply is_valid_for_reduce_correct; intuition.
-intro.
-rewrite forallb_forall in H.
-specialize (H t (all_list_forall t)).
-destruct (l t); intuition.
-apply is_valid_for_reduce_correct; intuition.
-Qed.
 
 (** The automaton is safe **)
 Definition safe :=
   shift_head_symbs /\ goto_head_symbs /\ shift_past_state /\
   goto_past_state /\ reduce_ok.
 
-Definition is_safe (_:unit) :=
-  (is_shift_head_symbs () && is_goto_head_symbs () && is_shift_past_state () &&
-    is_goto_past_state () && is_reduce_ok ())%bool.
-
-Property is_safe_correct:
-  is_safe () = true -> safe.
-Proof.
-unfold safe, is_safe.
-repeat rewrite Bool.andb_true_iff.
-intuition.
-apply is_shift_head_symbs_correct; assumption.
-apply is_goto_head_symbs_correct; assumption.
-apply is_shift_past_state_correct; assumption.
-apply is_goto_past_state_correct; assumption.
-apply is_reduce_ok_correct; assumption.
-Qed.
+Derive is_safe
+SuchThat (IsValidator safe (is_safe ()))
+As safe_is_validator.
+Proof. subst is_safe. instantiate (1:=fun _ => _). apply _. Qed.
 
 End Make.
